concurrency/README.md
@@ -6,8 +6,8 @@ It builds in Coq 8.8.0, by "make -kj7 concurrency" from the root directory.
 ---------------------------------------
 The main theorem is in concurrency/main.v:
 
-CSL2FineBareAsm_safety (* THE MAIN THEOREM *)
-  : forall
+    CSL2FineBareAsm_safety: (* THE MAIN THEOREM *)
+    forall
     (CPROOF : semax_to_juicy_machine.CSL_proof)
     (Asm_prog : Asm.program)
     (compilation: CC_correct.CompCert_compiler (Clight_prog CPROOF) =
@@ -36,119 +36,119 @@ CSL2FineBareAsm_safety (* THE MAIN THEOREM *)
             (HybridMachineSig.diluteMem init_mem_target') U n)
 
 Translation into English:
-  Suppose CPROOF is a derivation in Concurrent Separation Logic
-    that the program (Clight_prog := CSL_prog CPROOF) satisfies
-    the specification (CSL_G CPROOF).
-  Suppose [compilation] the CompCert compiler runs on Clight_prog,
-    producing Asm_prog.
-  Suppose [asm_genv_safe] that the only external "builtin" functions that
-    (statically) appear in the program are malloc/free/memcpy, or any
-    other function that does not modify memory.
-  Suppose [init_mem-wd] the initial memory state of the program (calculated by
-    CompCert's Genv.init_mem function) is well defined (this is
-    easy to statically check on any particular concrete program).
-  Suppose [CPROOF_initial] the initial Clight core state is a well-formed
-    start state for the entry point of the "main" function (has
-    appropriate formal parameter values, etc.).
-  Suppose [U] is an arbitrary preemptive schedule.
-  THEN
-  There exists an assembly-language initial memory [init_mem_target]
-    that is has all the initialized extern global variables as specified
-    in the program;
-  There exists a memory [init_mem_target'] that has in addition the stack frame
-    of the main function;
-  There exists an initial register bank [init_thread_target] at the entry    
-    of the main function;
-  We construct an initial thread pool [init_tp_target];
-  Such that [machine_semantics.initial_machine...] the machine state is
-    now a proper initial state for the program Asm_prog; and
-  For any number [n],
-  It is safe to run the fine-grain (preemptive) assembly language program
-     for n steps.
+
+    Suppose CPROOF is a derivation in Concurrent Separation Logic
+      that the program (Clight_prog := CSL_prog CPROOF) satisfies
+      the specification (CSL_G CPROOF).
+    Suppose [compilation] the CompCert compiler runs on Clight_prog,
+      producing Asm_prog.
+    Suppose [asm_genv_safe] that the only external "builtin" functions that
+      (statically) appear in the program are malloc/free/memcpy, or any
+      other function that does not modify memory.
+    Suppose [init_mem-wd] the initial memory state of the program (calculated by
+      CompCert's Genv.init_mem function) is well defined (this is
+      easy to statically check on any particular concrete program).
+    Suppose [CPROOF_initial] the initial Clight core state is a well-formed
+      start state for the entry point of the "main" function (has
+      appropriate formal parameter values, etc.).
+    Suppose [U] is an arbitrary preemptive schedule.
+    THEN
+    There exists an assembly-language initial memory [init_mem_target]
+      that is has all the initialized extern global variables as specified
+      in the program;
+    There exists a memory [init_mem_target'] that has in addition the
+      stack frame of the main function;
+    There exists an initial register bank [init_thread_target] at the entry    
+      of the main function;
+    We construct an initial thread pool [init_tp_target];
+    Such that [machine_semantics.initial_machine...] the machine state is
+      now a proper initial state for the program Asm_prog; and
+    For any number [n],
+    It is safe to run the fine-grain (preemptive) assembly language program
+       for n steps.
   
 ---------------------------------------
 
 The last line of concurrency/main.v is 
-Print Assumptions CSL2FineBareAsm_safety, which mentions the following
-axioms, categorized into
-  [R] part of the axiomatization of the Real numbers, which
-     we (involuntarily) inherit from CompCert's "Flocq" floating-point library
-  [A] axioms of logic known to be consistent with CiC (and each other)
-  [H] holes in our proof
-  [C] abstract parameters of CompCert, instantiated for any particular
-        machine such as x86_32
-  [B] bugs in Coq's print_assumptions command; see Coq issue #7192
-         https://github.com/coq/coq/issues/7192       
-  [D] The CompCert compiler itself
+Print Assumptions CSL2FineBareAsm_safety,
+which mentions the following axioms, categorized into
+    [A] axioms of logic known to be consistent with CiC (and each other)
+    [B] bugs in Coq's print_assumptions command; see Coq issue #7192
+           https://github.com/coq/coq/issues/7192       
+    [C] abstract parameters of CompCert, instantiated for any particular
+          machine such as x86_32
+    [D] The CompCert compiler itself
+    [R] part of the axiomatization of the Real numbers, used by
+        CompCert's "Flocq" floating-point library
+    [H] holes in our proof
 
-[R] Rdefinitions.up
-[R] Raxioms.total_order_T
-[H] BareMachine.syncstep_equal_run (Nick)
-[H] semax_ext.symb2genv_ax  (Andrew)
-[H] semax_ext.symb2genv  (Andrew) 
-[H] Asm.semantics_determinate (William and Nick)
-[A] Axioms.prop_ext
-[A] ProofIrrelevance.proof_irrelevance
-[A] lib.Axioms.proof_irr
-[H] safety.preservation  (Santiago)
-[H] enums_equality.ord_enum_enum (Andrew)
-[H] safety_equivalence.ksafe_csafe_equiv' (Santiago)
-[C] Events.inline_assembly_sem
-[H] x86_erasure.X86CoreErasure.inline_assembly_erasure (Nick)
-[H] ConcurCC_safe.initial_csafe_all_schedule (Santiago)
-[A] functional_extensionality_dep
-[B] SeparationLogicSoundness.SoundSeparationLogic.CSL.func_ptr_isptr
-[B] SeparationLogicSoundness.SoundSeparationLogic.CSL.func_ptr_def
-[B] SeparationLogicSoundness.SoundSeparationLogic.CSL.func_ptr
-[H] x86_erasure.X86CoreErasure.extsem_erasure (Nick)
-[C] Events.external_functions_sem
-[H] ConcurCC_safe.explicit_safety_step  (Santiago)
-[A] Eqdep.Eq_rect_eq.eq_rect_eq
-[H] X86Inj.corestep_wd  (Nick)
-[H] X86Inj.corestep_obs_eq (Nick)
-[H] x86_context.X86SEMAxioms.corestep_det (Nick) 
-[R] Raxioms.completeness
-[A] Classical_Prop.classic
-[R] Raxioms.archimed
-[B] SeparationLogicSoundness.SoundSeparationLogic.CSL.approx_func_ptr
-[B] safety.X_dec : forall (X : Type) (x y : X), {x = y} + {x <> y}
-[R] Raxioms.Rplus_opp_r
-[R] Raxioms.Rplus_lt_compat_l
-[R] Raxioms.Rplus_comm
-[R] Raxioms.Rplus_assoc
-[R] Raxioms.Rplus_0_l
-[R] Rdefinitions.Rplus
-[R] Rdefinitions.Ropp
-[R] Raxioms.Rmult_plus_distr_l
-[R] Raxioms.Rmult_lt_compat_l
-[R] Raxioms.Rmult_comm
-[R] Raxioms.Rmult_assoc
-[R] Raxioms.Rmult_1_l
-[R] Rdefinitions.Rmult
-[R] Raxioms.Rlt_trans
-[R] Raxioms.Rlt_asym
-[R] Rdefinitions.Rlt
-[R] Raxioms.Rinv_l
-[R] Rdefinitions.Rinv
-[R] Raxioms.R1_neq_R0
-[R] Rdefinitions.R1
-[R} Rdefinitions.R0
-[R] Rdefinitions.R
-[H] MemObsEq.EM : ClassicalFacts.excluded_middle (Nick)
-[H] ConcurCC_safe.ConcurCC_correct.ConcurrentCompilerCorrectness  (Santiago)
-[D] CC_correct.CompCert_compiler : program -> option Asm.program
-[H] Clight_safety.Clight_new_Clight_safety_gen  (William)
-[H] ConcurCC_safe.Clight_finite_branching  (Santiago)
-[H] ClightSemantincsForMachines.CLN_step_decay (Andrew)
-[H] ClightSemantincsForMachines.CLN_evsem_obligation_5 (Lennart)
-[H] ClightSemantincsForMachines.CLN_evsem_obligation_4 (Lennart)
-[H] ClightSemantincsForMachines.CLN_evsem_obligation_3 (Lennart)
-[H] ClightSemantincsForMachines.CLN_evsem_obligation_2 (Lennart)
-[H] ClightSemantincsForMachines.CLN_evsem_obligation_1 (Lennart)
-[H] ClightSemantincsForMachines.CLC_evsem_obligation_5 (Lennart)
-[H] ClightSemantincsForMachines.CLC_evsem_obligation_4 (Lennart)
-[H] ClightSemantincsForMachines.CLC_evsem_obligation_3 (Lennart)
-[H] ClightSemantincsForMachines.CLC_evsem_obligation_2 (Lennart)
-[H] ClightSemantincsForMachines.CLC_evsem_obligation_1 (Lennart)
   
-	
+    [R] Rdefinitions.up
+    [R] Raxioms.total_order_T
+    [H] BareMachine.syncstep_equal_run (Nick)
+    [H] semax_ext.symb2genv_ax  (Andrew)
+    [H] semax_ext.symb2genv  (Andrew) 
+    [H] Asm.semantics_determinate (William and Nick)
+    [A] Axioms.prop_ext
+    [A] ProofIrrelevance.proof_irrelevance
+    [A] lib.Axioms.proof_irr
+    [H] safety.preservation  (Santiago)
+    [H] enums_equality.ord_enum_enum (Andrew)
+    [H] safety_equivalence.ksafe_csafe_equiv' (Santiago)
+    [C] Events.inline_assembly_sem
+    [H] x86_erasure.X86CoreErasure.inline_assembly_erasure (Nick)
+    [H] ConcurCC_safe.initial_csafe_all_schedule (Santiago)
+    [A] functional_extensionality_dep
+    [B] SeparationLogicSoundness.SoundSeparationLogic.CSL.func_ptr_isptr
+    [B] SeparationLogicSoundness.SoundSeparationLogic.CSL.func_ptr_def
+    [B] SeparationLogicSoundness.SoundSeparationLogic.CSL.func_ptr
+    [H] x86_erasure.X86CoreErasure.extsem_erasure (Nick)
+    [C] Events.external_functions_sem
+    [H] ConcurCC_safe.explicit_safety_step  (Santiago)
+    [A] Eqdep.Eq_rect_eq.eq_rect_eq
+    [H] X86Inj.corestep_wd  (Nick)
+    [H] X86Inj.corestep_obs_eq (Nick)
+    [H] x86_context.X86SEMAxioms.corestep_det (Nick) 
+    [R] Raxioms.completeness
+    [A] Classical_Prop.classic
+    [R] Raxioms.archimed
+    [B] SeparationLogicSoundness.SoundSeparationLogic.CSL.approx_func_ptr
+    [B] safety.X_dec : forall (X : Type) (x y : X), {x = y} + {x <> y}
+    [R] Raxioms.Rplus_opp_r
+    [R] Raxioms.Rplus_lt_compat_l
+    [R] Raxioms.Rplus_comm
+    [R] Raxioms.Rplus_assoc
+    [R] Raxioms.Rplus_0_l
+    [R] Rdefinitions.Rplus
+    [R] Rdefinitions.Ropp
+    [R] Raxioms.Rmult_plus_distr_l
+    [R] Raxioms.Rmult_lt_compat_l
+    [R] Raxioms.Rmult_comm
+    [R] Raxioms.Rmult_assoc
+    [R] Raxioms.Rmult_1_l
+    [R] Rdefinitions.Rmult
+    [R] Raxioms.Rlt_trans
+    [R] Raxioms.Rlt_asym
+    [R] Rdefinitions.Rlt
+    [R] Raxioms.Rinv_l
+    [R] Rdefinitions.Rinv
+    [R] Raxioms.R1_neq_R0
+    [R] Rdefinitions.R1
+    [R} Rdefinitions.R0
+    [R] Rdefinitions.R
+    [H] MemObsEq.EM : ClassicalFacts.excluded_middle (Nick)
+    [H] ConcurCC_safe.ConcurCC_correct.ConcurrentCompilerCorrectness  (Santiago)
+    [D] CC_correct.CompCert_compiler : program -> option Asm.program
+    [H] Clight_safety.Clight_new_Clight_safety_gen  (William)
+    [H] ConcurCC_safe.Clight_finite_branching  (Santiago)
+    [H] ClightSemantincsForMachines.CLN_step_decay (Andrew)
+    [H] ClightSemantincsForMachines.CLN_evsem_obligation_5 (Lennart)
+    [H] ClightSemantincsForMachines.CLN_evsem_obligation_4 (Lennart)
+    [H] ClightSemantincsForMachines.CLN_evsem_obligation_3 (Lennart)
+    [H] ClightSemantincsForMachines.CLN_evsem_obligation_2 (Lennart)
+    [H] ClightSemantincsForMachines.CLN_evsem_obligation_1 (Lennart)
+    [H] ClightSemantincsForMachines.CLC_evsem_obligation_5 (Lennart)
+    [H] ClightSemantincsForMachines.CLC_evsem_obligation_4 (Lennart)
+    [H] ClightSemantincsForMachines.CLC_evsem_obligation_3 (Lennart)
+    [H] ClightSemantincsForMachines.CLC_evsem_obligation_2 (Lennart)
+    [H] ClightSemantincsForMachines.CLC_evsem_obligation_1 (Lennart)
